Substitutions.dfy
@@ -1,16 +1,16 @@
+include "Definitions.dfy"
 /*
  * Substitutes all occurances of v in X in S with v' in X'
  * 
  */
 function method substitute(S: Statement, X: seq<Variable>, X': seq<Variable>) : (S': Statement)
+reads *
 requires Valid(S)
 requires |X| == |X'|
 requires setOf(X) !! setOf(X')
-requires setOf(X) <= glob(S)
-requires setOf(X') !! glob(S) // consider replacing with allVars(S) (including locals)
-requires S.Skip? || S.Assignment? || S.SeqComp? || S.IF? || S.DO? // replace with Core(S)
-ensures setOf(X') <= glob(S')
-ensures setOf(X) !! glob(S)
+requires setOf(X') !! allVars(S)
+requires Core(S)
+ensures setOf(X) !! allVars(S')
 ensures Valid(S')
 {
 	match S {
@@ -18,86 +18,109 @@ ensures Valid(S')
 		case Assignment(LHS, RHS) => 
 			var LHS' := VSubstitute(LHS, X, X');
 			var RHS' := ESeqSubstitute(RHS, X, X');
-			Assignment(LHS', RHS');
+			assert |LHS'| == |RHS'|;
+			Assignment(LHS', RHS')
 		case SeqComp(S1, S2) => 
 			var S1' := substitute(S1, X, X');
 			var S2' := substitute(S2, X, X');
 			SeqComp(S1', S2')
 		case IF(B0, Sthen, Selse) => 
-			var B' := BSubstitue(B0, X, X');
+			var B' := BSubstitute(B0, X, X');
 			var Sthen' := substitute(Sthen, X, X');
 			var Selse' := substitute(Selse, X, X');
 			IF(B', Sthen', Selse')
 		case DO(B, S) => 
-			var B' := BSubstitue(B, X, X');
+			var B' := BSubstitute(B, X, X');
 			var S'' := substitute(S, X, X');
 			DO(B', S'')
 
 		case LocalDeclaration(L, S0) => Skip // S is Core Statement
-		case Live(L, S0) => Skip // S is Core Statement
+		//case Live(L, S0) => Skip // S is Core Statement
 	}
 }
 
 function method {:verify true} VSubstitute(
 	LHS: seq<Variable>,
 	X: seq<Variable>,
-	X': seq<Variable>): seq<Variable>
+	X': seq<Variable>): (res: seq<Variable>)
 	requires |X| == |X'|
+	requires setOf(X) !! setOf(X')
+	ensures |res| == |LHS|
+	ensures setOf(X) !! setOf(res)
 {
 	if LHS == [] then []
 	else
 		[if LHS[0] in X
-			then GetCorrespondingV(LHS[0], X, X');
+			then GetCorrespondingV(LHS[0], X, X')
 			else LHS[0]] 
 		 + VSubstitute(LHS[1..], X, X')
 }
 
-function method {:verify true} GetCorrespondingV(v: Variable, X: seq<Variable, X': seq<Variable): Variable
+function method {:verify true} GetCorrespondingV(v: Variable, X: seq<Variable>, X': seq<Variable>)
+: (res: Variable)
 	requires v in X
 	requires |X| == |X'|
+	requires setOf(X) !! setOf(X')
+	ensures res in X'
 {
 	if v == X[0] then X'[0]
 	else
+		assert setOf(X[1..]) !! setOf(X'[1..]) by {
+			assert setOf(X[1..]) <= setOf(X);
+		}
 		GetCorrespondingV(v, X[1..], X'[1..])
 }
 
-function method {:verify true} BSubstitue(
+function method {:verify true} BSubstitute(
 	B0: BooleanExpression,
 	X: seq<Variable>,
-	X': seq<Variable>) : BooleanExpression
+	X': seq<Variable>) : (res: BooleanExpression)
+reads *
+requires |X| == |X'|
+requires setOf(X) !! setOf(X')
+ensures |B0.1-setOf(X)+setOf(X')|==|res.1|
+ensures setOf(X) !! res.1
 {
-	(state=>
-		B0.0(map v | v in (B0.1-setOf(X)+setOf(X')) :: 
-				(if v !in X' 
+	((state reads * requires(forall v :: v in B0.1-setOf(X)+setOf(X') ==> v in state)
+		requires forall m :: (forall v :: v in B0.1 ==> v in m) ==> B0.0.requires(m) 
+		=> 
+			var m := map v | v in B0.1 :: 
+			(if v !in X 	
 				then state[v] 
-				else state[FindParallelV(v, X, X')])
-			),
-		B0.1-setOf(X)+setOf(X'))
+				else state[FindParallelV(v, X, X')]);
+
+		B0.0(m)),
+	 B0.1-setOf(X)+setOf(X'))
 }
 
-function method {:verify true} ESubstitue(
+function method {:verify true} ESubstitute(
 	E: Expression,
 	X: seq<Variable>,
 	X': seq<Variable>) : (res:Expression)
-requires |X| <= |X'|
-ensures |E.1|==|res.1|
+reads *
+requires |X| == |X'|
+requires setOf(X) !! setOf(X')
+ensures |E.1-setOf(X)+setOf(X')|==|res.1|
+ensures setOf(X) !! res.1
 {
-	(state=>
-		E.0(map v | v in (E.1-setOf(X)+setOf(X')) :: 
-				(if v !in X' 	
+	((state reads * requires(forall v :: v in E.1-setOf(X)+setOf(X') ==> v in state)
+		requires forall m :: (forall v :: v in E.1 ==> v in m) ==> E.0.requires(m) 
+		=> 
+			var m := map v | v in E.1 :: 
+			(if v !in X 	
 				then state[v] 
-				else state[FindParallelV(v, X, X')])
-			),
-		E.1-setOf(X)+setOf(X'))
+				else state[FindParallelV(v, X, X')]);
+
+		E.0(m)),
+	 E.1-setOf(X)+setOf(X'))
 }
 
 function method {:verify true} FindParallelV(v: Variable,
 	X: seq<Variable>,
-	X': seq<Variable>) : Variable
-requires |X| > 0
-requires |X'| > 0
-requires |X| <= |X'|
+	X': seq<Variable>) : (res: Variable)
+requires |X| == |X'|
 requires v in X
+ensures res in X'
 {
 	if v == X[0] then X'[0] else
 	FindParallelV(v, X[1..], X'[1..])
@@ -107,9 +130,13 @@ function method {:verify true} ESeqSubstitute(
 	Es : seq<Expression>,
 	X: seq<Variable>,
 	X': seq<Variable>) : (res : seq<Expression>)
-requires |X| <= |X'|
+reads *
+requires |X| == |X'|
+requires setOf(X) !! setOf(X')
+ensures |res| == |Es|
+ensures setOf(X) !! varsInExps(res)
 {
 	if Es == [] then []
 	else
-		[ESubstitue(Es[0], X, X')]+ESeqSubstitute(Es[1..], X, X')
+		[ESubstitute(Es[0], X, X')]+ESeqSubstitute(Es[1..], X, X')
 }
